This version of Smtlink doesn't run. I'm trying to make some big change of removing fixing functions from Smtlink.lisp. I figured it might be better to remember what they used to be, in case I find out that I need them in the end.

verified/Smtlink.lisp
@@ -8,9 +8,11 @@
 (in-package "SMT")
 (include-book "std/util/bstar" :dir :system)
 (include-book "std/util/define" :dir :system)
+(include-book "std/basic/inductions" :dir :system)
 
 (include-book "SMT-hint-interface")
 (include-book "SMT-verified-cps")
+(include-book "SMT-config")
 
 ;; (defsection Smtlink-process-user-hint
 ;;   :parents (Smtlink)
@@ -19,62 +21,546 @@
 
   ;; --------------------------------------------------------
 
-  ;; Example:
-  ;; (defthm ...
-  ;;   ...
-  ;;   :hints (("Goal"
-  ;;            :clause-processor
-  ;;            (SMT::smtlink clause
-  ;;                          '(:functions ()
-  ;;                            :hypotheses ()
-  ;;                            :main-hint ()
-  ;;                            :int-to-rat nil
-  ;;                            :smt-fname ""
-  ;;                            :rm-file t
-  ;;                            :smt-solver-params ()
-  ;;                            :smt-cnf ())))))
+;; Example:
+;; :hints (("Goal"
+;;          :clause-processor
+;;          (SMT::smtlink clause
+;;                        '(:functions ((f0 :formals ((a0 rationalp))
+;;                                          :returns (r0 rationalp :hints (:use ((:instance returns-lemma))))
+;;                                          :level 1
+;;                                          :guard ((> a0 0) :hints (:use ((:instance guard-lemma))))
+;;                                          :more-returns ((> r0 0) :hints (:use ((:instance more-lemma))))))
+;;                          :hypothesis (((> a b) :hints (:use ((:instance lemma)))))
+;;                          :main-hint (:use ((:instance thm1)))
+;;                          :int-to-rat nil
+;;                          :smt-fname ""
+;;                          :rm-file t
+;;                          :smt-solver-params (...)
+;;                          :smt-cnf ()))))
+;;
+;; Types:
+;; qbooleanp/error
+;; qnatp/error
+;; qstringp/error
+;; hints-syntax-p/error
+;; hypothesis-syntax-p/error
+;; hypothesis-lst-syntax-p/error
+;; argument-syntax-p/error
+;; argument-lst-syntax-p/error
+;; function-option-syntax-p/error
+;; function-option-lst-syntax-p/error
+;; function-syntax-p/error
+;; function-lst-syntax-p/error
+;; smtlink-cnf-p/error
+;; smt-solver-params-p/error
+;; smtlink-hint-syntax-p/error
 
-  (define true-list-fix ((lst t))
-    :short "Fixing function for true-listp."
-    :returns (fixed-lst true-listp)
-    (if (true-listp lst)
-        lst
-      nil))
+(define true-list-fix ((lst t))
+  :short "Fixing function for true-listp."
+  :returns (fixed-lst true-listp)
+  (if (true-listp lst)
+      lst
+    nil))
 
-  (defconst *syntax-lst*
-    '((:functions . listp)
-      (:hypotheses . listp)
-      (:main-hint . listp)
-      (:int-to-rat . booleanp)
-      (:smt-fname . stringp)
-      (:rm-file . booleanp)
-      (:smt-solver-params . listp)
-      (:smt-cnf . listp)))
+(define qstringp ((term t))
+  :returns (syntax-good? booleanp)
+  :short "Recognizer for a quoted stringp."
+  (and (true-listp term)
+       (equal (len term) 2)
+       (equal (car term) 'quote)
+       (stringp (cadr term))))
+
+(define qstring-fix ((term qstringp))
+  :short "Fixing function for a qstringp."
+  :returns (fixed-qstring qstringp)
+  (mbe :logic (if (qstringp term) term ''"")
+       :exec term))
+
+(define qnatp ((term t))
+  :returns (syntax-good? booleanp)
+  :short "Recognizer for a quoted qnatp."
+  (and (true-listp term)
+       (equal (len term) 2)
+       (equal (car term) 'quote)
+       (natp (cadr term))))
+
+(define qnat-fix ((term qnatp))
+  :returns (fixed-qnat qnatp)
+  :short "Fixing function for a qnatp."
+  (mbe :logic (if (qnatp term) term ''0)
+       :exec term))
+
+(define qbooleanp ((term t))
+  :short "Recognizer for a quoted booleanp."
+  :returns (syntax-good? booleanp)
+  (and (true-listp term)
+       (equal (len term) 2)
+       (equal (car term) 'quote)
+       (booleanp (cadr term))))
+
+(define qboolean-fix ((term qbooleanp))
+  :returns (fixed-qboolean qbooleanp)
+  :short "Fixing function for a qbooleanp."
+  (mbe :logic (if (qbooleanp term) term ''nil)
+       :exec term))
+
+(define hints-syntax-p ((term t))
+  :returns (syntax-good? booleanp)
+  :short "Recognizer for hints-syntax."
+  (true-listp term))
+
+(define hints-syntax-fix ((term hints-syntax-p))
+  :returns (fixed-hints-syntax hints-syntax-p)
+  :short "Fixing function for a hints-sytnax-p."
+  (mbe :logic (if (hints-syntax-p term) term nil)
+       :exec term))
+
+(define hypothesis-syntax-p ((term t))
+  :returns (syntax-good? booleanp)
+  :short "Recognizer for hypothesis-syntax."
+  (or (and (atom term)
+           (equal term nil))
+      ;; Without hints
+      (and (true-listp term)
+           (equal (len term) 1)
+           (pseudo-termp (car term)))
+      ;; With hints
+      (and (true-listp term)
+           (equal (len term) 3)
+           (pseudo-termp (car term))
+           (equal (cadr term) ':hints)
+           (hints-syntax-p (caddr term)))))
+
+(define hypothesis-syntax-fix ((term hypothesis-syntax-p))
+  :returns (fixed-hypothesis hypothesis-syntax-p)
+  :short "Fixing function for a hypothesis-syntax-p."
+  (mbe :logic (if (hypothesis-syntax-p term) term nil)
+       :exec term))
+
+(define hypothesis-lst-syntax-p ((term t))
+  :returns (syntax-good? booleanp)
+  :short "Recognizer for hypothesis-lst-syntax."
+  (b* (((if (atom term)) (equal term nil))
+       ((cons first rest) term))
+    (and (hypothesis-syntax-p first)
+         (hypothesis-lst-syntax-p rest))))
+
+(define hypothesis-lst-syntax-fix ((term hypothesis-lst-syntax-p))
+  :returns (fixed-hypothesis-lst-syntax hypothesis-lst-syntax-p
+                                        :hints (("Goal"
+                                                 :in-theory (enable hypothesis-lst-syntax-p))))
+  :verify-guards nil
+  :short "Fixing function for a hypothesis-lst-syntax-p."
+  (mbe :logic (if (consp term)
+                  (cons (hypothesis-syntax-fix (car term))
+                        (hypothesis-lst-syntax-fix (cdr term)))
+                nil)
+       :exec term))
+
+(verify-guards hypothesis-lst-syntax-fix
+  :hints (("Goal" :in-theory (enable hypothesis-syntax-fix
+  hypothesis-lst-syntax-p hypothesis-lst-syntax-fix))))
+
+(define smt-typep ((term t))
+  :returns (valid-type? booleanp)
+  :short "Types allowed in Smtlink."
+  (if (member-equal term
+                    ' (rationalp realp rational/realp booleanp integerp))
+      t nil))
+
+(define argument-syntax-p ((term t))
+  :returns (syntax-good? booleanp)
+  :short "Recognizer for argument-syntax."
+  (or (and (atom term)
+           (equal term nil))
+      ;; Just the name
+      (and (true-listp term)
+           (equal (len term) 1)
+           (symbolp (car term)))
+      ;; The name and the type/guard
+      (and (true-listp term)
+           (equal (len term) 2)
+           (smt-typep (car term))
+           (pseudo-termp (cadr term)))
+      ;; The name, the type and the :hints
+      (and (true-listp term)
+           (equal (len term) 3)
+           (symbolp (car term))
+           (smt-typep (cadr term))
+           (hints-syntax-p (cddr term)))))
+
+(define argument-syntax-fix ((term argument-syntax-p))
+  :returns (fixed-argument-syntax argument-syntax-p)
+  :short "Fixing function for argument-syntax-p."
+  (mbe :logic (if (argument-syntax-p term) term nil)
+       :exec term))
+
+(define argument-lst-syntax-p ((term t))
+  :short "Recognizer for argument-lst-syntax."
+  :returns (syntax-good? booleanp)
+  (b* (((if (atom term)) (equal term nil))
+       ((cons first rest) term))
+    (and (argument-syntax-p first)
+         (argument-lst-syntax-p rest))))
+
+(define argument-lst-syntax-fix ((term argument-lst-syntax-p))
+  :short "Fixing function for argument-lst-syntax."
+  :returns (fixed-argument-lst-syntax argument-lst-syntax-p
+                                      :hints (("Goal"
+                                               :in-theory (enable argument-lst-syntax-p))))
+  :verify-guards nil
+  (mbe :logic (if (consp term)
+                  (cons (argument-syntax-fix (car term))
+                        (argument-lst-syntax-fix (cdr term)))
+                nil)
+       :exec term))
+(verify-guards argument-lst-syntax-fix
+  :hints (("Goal"
+           :in-theory (enable argument-lst-syntax-fix argument-syntax-fix argument-lst-syntax-p))))
+
+(defconst *function-option*
+  '((:formals . argument-lst-syntax-p)
+    (:returns . argument-lst-syntax-p)
+    (:level . qnatp)
+    (:guard . hypothesis-lst-syntax-p)
+    (:more-returns . hypothesis-lst-syntax-p)))
+
+(defconst *option-type*
+  (strip-cdrs *function-option*))
+
+(define function-option-p ((term t))
+  :returns (syntax-good? booleanp)
+  :short "Recoginizer for function-option."
+  (if (assoc-equal term *function-option*) t nil))
+
+(define option-type-p ((option t))
+  :returns (syntax-good? booleanp)
+  :short "Recoginizer for option-type."
+  (if (member-equal option *option-type*) t nil))
+
+(define option-type-lst-p ((option-lst t))
+  :returns (syntax-good? booleanp)
+  :short "Recoginizer for option-type-lst."
+  (b* (((if (atom option-lst)) (equal option-lst nil))
+       ((cons first rest) option-lst))
+    (and (option-type-p first)
+         (option-type-lst-p rest))))
+
+;; The conditions in eval-type should go along with *function-option*
+(define eval-type ((option-type option-type-p) (term t))
+  :returns (type-cuorrect? booleanp)
+  :short "Evaluating types for function option body."
+  (case option-type
+    (:formals (argument-lst-syntax-p term))
+    (:returns (argument-lst-syntax-p term))
+    (:level (qnatp term))
+    (:guard (hypothesis-lst-syntax-p term))
+    (t (hypothesis-lst-syntax-p term))))
+
+(define function-option-syntax-p ((term t) (used option-type-lst-p))
+  :returns (syntax-good? booleanp)
+  :short "Recoginizer for function-option-syntax."
+  :verify-guards nil
+  (b* (((if (equal term nil)) t)
+       ((unless (and (true-listp term) (equal (len term) 2))) nil)
+       ((cons option body-lst) term)
+       ((unless (function-option-p option)) nil)
+       (option-type (cdr (assoc-equal option *function-option*))))
+    (and (not (member-equal option used))
+         (eval-type option-type (car body-lst)))))
+(verify-guards function-option-syntax-p
+  :guard-debug t
+  :hints (("Goal" :in-theory (enable function-option-syntax-p function-option-p
+                                     eval-type option-type-lst-p))))
+
+(define function-option-syntax-fix ((term function-option-syntax-p) (used option-type-lst-p))
+  :returns (fixed-function-option-syntax function-option-syntax-p)
+  :short "Fixing function for function-option-syntax."
+  (mbe :logic (if (function-option-syntax-p term used) term nil)
+       :exec term))
+
+(define function-option-lst-syntax-p (())
+  :returns ())
+(define function-option-lst-syntax-fix ())
+
+(define function-syntax-p ((term t))
+  :returns (syntax-good? booleanp)
+  :short "Recognizer for function-syntax."
+  (b* (((unless (true-listp term)) nil)
+       ((unless (consp term)) t)
+       ((cons fname function-options) term))
+    ;; It's probably possible to check existence of function?
+    ;; Currently not doing such check, since it will require passing state.
+    (and (symbolp fname)
+         (function-option-lst-syntax-p function-options))))
+
+(define function-syntax-fix ((term function-syntax-p))
+  :returns (fixed-function-syntax function-syntax-p)
+  :short "Fixing function for function-syntax."
+  ())
+
+(define function-lst-syntax-fix)
+(define function-lst-syntax-p)
+
+(define smtlink-hint-syntax-fix)
+(define smtlink-hint-syntax-p)
+
+(defconst *func-specs-syntax-lst*
+  '((:formals . p)
+    (:returns . p)
+    (:level . qnatp)
+    (:guard . p)
+    (:more-returns . p)))
 
   (define eval-type ((type symbolp) (content t))
     :short "Evaluate if a content is of the given type."
     :returns (type-correct? booleanp)
     (cond ((equal type 'booleanp) (booleanp content))
           ((equal type 'stringp) (stringp content))
-          ((equal type 'listp) (listp content))
+          ((equal type 'true-listp) (true-listp content))
+          ((equal type 'natp) (natp content))
+          ((equal type 'smtlink-config-p) (smtlink-config-p content))
           (t (symbolp content))))
+
+(define hint-pair-syntax-p ((hint-pair t))
+  :returns (syntax-good? booleanp)
+  (or (and (equal (len hint-pair) 3) (symbolp (car hint-pair))
+           (equal (cadr hint-pair) ':hints) (listp (caddr hint-pair)))
+      (and (equal (len hint-pair) 1) (symbolp (car hint-pair)))))
+
+  (define save-hint-pair-list ((hypo-lst true-listp))
+    :returns (saved-hypo-lst hint-pair-listp)
+    :measure (len hypo-lst)
+    :hints (("Goal" :in-theory (enable true-list-fix)))
+    :verify-guards nil
+    (b* ((hypo-lst (true-list-fix hypo-lst))
+         ((unless (consp hypo-lst)) nil)
+         ((cons first rest) hypo-lst)
+         ((unless (hint-pair-syntax-p first))
+          (er hard? 'Smtlink=>save-hint-pair-list "Wrong format of Smtlink-hint
+  hint-pair: ~q0" first))
+         ((cons thm hints) first))
+      (cons (case-match
+              hints
+              ((':hints hints) (make-hint-pair :thm thm :hints hints))
+              (& (make-hint-pair :thm thm)))
+            (save-hint-pair-list rest))))
+
+(verify-guards save-hint-pair-list
+  :hints (("Goal" :in-theory (enable hint-pair-syntax-p))))
+
+  (define decl-syntax-p ((decl t))
+    :returns (syntax-good? booleanp)
+    (or (and (equal (len decl) 4) (symbolp (car decl))
+             (hint-pair-syntax-p (cdr decl)))
+        (and (equal (len decl) 2) (symbolp (car decl))
+             (hint-pair-syntax-p (cdr decl)))))
+
+;; This function requires supper long proof.
+(define save-decl-list ((decl-lst true-listp))
+  :returns (saved-decl-lst decl-listp)
+  :measure (len decl-lst)
+  :hints (("Goal" :in-theory (enable true-list-fix)))
+  :verify-guards nil
+  (b* ((decl-lst (true-list-fix decl-lst))
+       ((unless (consp decl-lst)) nil)
+       ((cons first rest) decl-lst)
+       ((unless (decl-syntax-p first))
+        (er hard? 'Smtlink=>save-decl-list "Wrong format of Smtlink-hint decl:
+  ~q0" first))
+       ((cons name (cons type hint-pair)) first)
+       (hint-pair (case-match
+                    hint-pair
+                    ((':hints hints) (make-hint-pair :thm type :hints hints))
+                    (& (make-hint-pair :thm type)))))
+    (cons (make-decl :name name :type hint-pair)
+          (save-decl-list rest))))
+
+(verify-guards save-decl-list
+  :hints (("Goal" :in-theory (enable decl-syntax-p hint-pair-syntax-p))))
+
+
+(define check-func-specs-syntax ((func-spec-lst true-listp) (used true-listp))
+  :returns (syntax-good? booleanp)
+  :hints (("Goal" :in-theory (enable true-list-fix)))
+  (b* ((func-spec-lst (true-list-fix func-spec-lst))
+       (used (true-list-fix used))
+       ((if (endp func-spec-lst)) t)
+       ((unless (and (car func-spec-lst) (cadr func-spec-lst))) nil)
+       ((cons first rest) func-spec-lst)
+       ((cons second rest-of-second) rest)
+       ((if (member-equal first used))
+        (er hard? 'Smtlink=>check-func-specs-syntax "Already defined ~p0.~%" first))
+       (exist? (assoc-equal first *func-specs-syntax-lst*))
+       ((unless exist?) nil)
+       (type (cdr exist?))
+       (type-correct? (eval-type type second))
+       ((unless type-correct?) nil))
+    (check-func-specs-syntax rest-of-second (cons first used)))
+  ///
+  (skip-proofs
+   (defthm test
+     (IMPLIES (AND (CHECK-FUNC-SPECS-SYNTAX OTHER NIL))
+              (CHECK-FUNC-SPECS-SYNTAX (CDDR OTHER) NIL))))
+
+  (defthm check-func-specs-syntax-natp
+    (implies (and (true-listp other)
+                  (check-func-specs-syntax other nil)
+                  (equal (car other) :level))
+             (natp (cadr other)))
+    :hints (("Goal" :in-theory (enable true-list-fix eval-type))))
+
+  (defthm check-func-specs-syntax-true-listp
+    (implies (and (true-listp other)
+                  (check-func-specs-syntax other nil)
+                  (or (equal (car other) :formals)
+                      (equal (car other) :more-returns)
+                      (equal (car other) :guard)
+                      (equal (car other) :returns)))
+             (true-listp (cadr other)))
+    :hints (("Goal" :in-theory (enable true-list-fix eval-type))))
+  )
+
+(define func-specs-syntax-p ((func-specs t))
+  :returns (syntax-good? booleanp)
+  (b* (((unless (true-listp func-specs)) nil)
+       ((unless (<= (len func-specs) 10)) nil))
+    (check-func-specs-syntax func-specs nil)))
+
+(define func-specs-syntax-fix ((func-specs func-specs-syntax-p))
+  :returns (fixed-func-specs func-specs-syntax-p)
+  (if (func-specs-syntax-p func-specs) func-specs nil))
+
+(define save-a-function ((name symbolp) (other func-specs-syntax-p) (func func-p))
+  :returns (saved-func func-p)
+  :measure (len other)
+  :verify-guards nil
+  :hints (("Goal" :in-theory (enable func-specs-syntax-fix)))
+  (b* ((name (symbol-fix name))
+       (other (func-specs-syntax-fix other))
+       ((unless (consp other)) (make-func))
+       ((cons first rest) other)
+       ((cons second rest-of-second) rest))
+    (case first
+      (:formals
+       (save-a-function name rest-of-second
+                        (change-func func :formals (save-decl-list second))))
+      (:guard
+       (save-a-function name rest-of-second
+                        (change-func func :guard (save-hint-pair-list second))))
+      (:returns
+       (save-a-function name rest-of-second
+                        (change-func func :returns (save-decl-list second))))
+      (:more-returns
+       (save-a-function name rest-of-second
+                        (change-func func :more-returns (save-hint-pair-list second))))
+      (:level
+       (save-a-function name rest-of-second
+                        (change-func func :expansion-depth second)))
+      (t (prog2$
+          (er hard? 'Smtlink=>save-a-function "Functions hint in Smtlink hint
+  seems in the wrong format ~p0.~%" other)
+          (make-func))))))
+
+(verify-guards save-a-function
+  :hints (("Goal" :in-theory (enable func-specs-syntax-fix func-specs-syntax-p
+  eval-type assoc-equal check-func-specs-syntax)))
+  :guard-debug t)
+
+(define func-syntax-p ((func t))
+  :returns (syntax-good? booleanp)
+  (and (true-listp func)
+       (symbolp (car func))
+       (func-specs-syntax-p (cdr func))))
+
+(define save-functions ((func-lst true-listp))
+  :returns (saved-funcs func-alistp
+                        :hints (("Goal" :in-theory (enable true-list-fix func-syntax-p))))
+  :measure (len func-lst)
+  :hints (("Goal" :in-theory (enable true-list-fix)))
+  :verify-guards nil
+  (b* ((func-lst (true-list-fix func-lst))
+       ((unless (consp func-lst)) nil)
+       ((cons first rest) func-lst)
+       ((unless (func-syntax-p first))
+        (prog2$
+         (er hard? 'Smtlink=>save-functions "Wrong syntax for Smtlink function
+  declaration ~q0" first)
+         nil))
+       ((cons name other) first)
+       (saved-func (save-a-function name other (make-func))))
+    (cons (cons name saved-func)
+          (save-functions rest))))
+
+(verify-guards save-functions
+  :guard-debug t
+  :hints (("Goal" :in-theory (enable func-syntax-p))))
+
 
   (define check-syntax ((hint-lst true-listp) (used true-listp))
     :short "Main function for checking the syntax of a Smtlink hint list."
     :returns (syntax-good? booleanp)
     :hints (("Goal" :in-theory (enable true-list-fix)))
     (b* ((hint-lst (true-list-fix hint-lst))
-         ((if (endp hint-lst)) t)
-         ((cons first rest) hint-lst)
+         ((unless (consp hint-lst)) t)
+         ((cons kwd rest) hint-lst)
+         ((unless (consp rest)) (er hard? 'Smtlink=>check-syntax "wrong syntax ~p0.~%" hint-lst))
          ((cons second rest-of-second) rest)
-         ((if (member-equal first used))
-          (er hard? 'Smtlink=>check-syntax "Already defined ~p0.~%" first))
-         (exist? (assoc-equal first *syntax-lst*))
-         ((unless exist?) nil)
-         (type (cdr exist?))
-         (type-correct? (eval-type type second))
-         ((unless type-correct?) nil))
-      (check-syntax rest-of-second (cons first used))))
+         ((if (member-equal kwd used))
+          (er hard? 'Smtlink=>check-syntax "Already defined ~p0.~%" kwd))
+         (exist? (assoc-equal kwd *syntax-lst*))
+         ((unless exist?) (er hard? 'Smtlink=>check-syntax "unrecognized keyword ~p0.~%" kwd))
+         ;; (type (cdr exist?))
+         ;; (type-correct? (eval-type type second))
+         ;; ((unless type-correct?) nil)
+         )
+      (check-syntax rest-of-second (cons first used)))
+    ///
+    (defthm check-syntax-cddr-lemma
+      (implies (check-syntax user-hints lst)
+               (check-syntax user-hints nil))
+      :hints (("Goal"
+               :in-theory (enable true-list-fix)
+               :cases (member-euqla first used)
+               )))
+
+    (defthm check-syntax-cddr
+      (implies (check-syntax user-hints nil)
+               (check-syntax (cddr user-hints) nil))
+      :hints (("Goal" :in-theory (enable true-list-fix))))
+
+    (defthm check-syntax-true-listp
+      (implies (and (true-listp hint-lst)
+                    (check-syntax hint-lst nil)
+                    (or (equal (car hint-lst) :functions)
+                        (equal (car hint-lst) :hypotheses)
+                        (equal (car hint-lst) :main-hint)
+                        (equal (car hint-lst) :smt-solver-params)))
+               (true-listp (cadr hint-lst)))
+      :hints (("Goal" :in-theory (enable true-list-fix eval-type))))
+
+    (defthm check-syntax-smtlink-config-p
+      (implies (and (true-listp hint-lst)
+                    (check-syntax hint-lst nil)
+                    (equal (car hint-lst) :smt-cnf))
+               (smtlink-config-p (cadr hint-lst)))
+      :hints (("Goal" :in-theory (enable true-list-fix eval-type))))
+
+    (defthm check-syntax-booleanp
+      (implies (and (true-listp hint-lst)
+                    (check-syntax hint-lst nil)
+                    (or (equal (car hint-lst) :int-to-rat)
+                        (equal (car hint-lst) :rm-file)))
+               (booleanp (cadr hint-lst)))
+      :hints (("Goal" :in-theory (enable true-list-fix eval-type))))
+
+    (defthm check-syntax-stringp
+      (implies (and (true-listp hint-lst)
+                    (check-syntax hint-lst nil)
+                    (equal (car hint-lst) :smt-fname))
+               (stringp (cadr hint-lst)))
+      :hints (("Goal" :in-theory (enable true-list-fix eval-type))))
+    )
 
   (define smtlink-hint-syntax-p ((hint-lst t))
     :short "Syntax check for Smtlink hint."
@@ -92,15 +578,156 @@
     :irrelevant-formals-ok t
     (if (smtlink-hint-syntax-p hint-lst) hint-lst nil))
 
+(define save-user-hints ((user-hints smtlink-hint-syntax-p) (the-hint smtlink-hint-p))
+  :returns (structured-hint maybe-smtlink-hint-p)
+  :measure (len user-hints)
+  :hints (("Goal" :in-theory (enable smtlink-hint-syntax-fix)))
+  :verify-guards nil
+  (b* ((user-hints (smtlink-hint-syntax-fix user-hints))
+       ((unless (consp user-hints)) nil)
+       (the-hint (smtlink-hint-fix the-hint))
+       ((cons first rest) user-hints)
+       ((cons second rest-of-second) rest))
+    (case first
+      (:functions
+       (save-user-hints rest-of-second
+                        (change-smtlink-hint the-hint :user-functions (save-functions second))))
+      (:hypotheses
+       (save-user-hints rest-of-second
+                        (change-smtlink-hint the-hint :hypotheses (save-hint-pair-list second))))
+      (:main-hint
+       (save-user-hints rest-of-second
+                        (change-smtlink-hint the-hint :main-hint second)))
+      (:int-to-rat
+       (save-user-hints rest-of-second
+                        (change-smtlink-hint the-hint :int-to-rat second)))
+      (:smt-fname
+       (save-user-hints rest-of-second
+                        (change-smtlink-hint the-hint :smt-fname second)))
+      (:rm-file
+       (save-user-hints rest-of-second
+                        (change-smtlink-hint the-hint :rm-file second)))
+      (:smt-solver-params
+       (save-user-hints rest-of-second
+                        (change-smtlink-hint the-hint :smt-params second)))
+      (:smt-cnf
+       (save-user-hints rest-of-second
+                        (change-smtlink-hint the-hint :smt-cnf second)))
+      ;; :smt-cnf
+      ;; There might be problems with the merge of smt-cnf.
+      ;; I'm assuming smt-cnf is already in its correct form.
+      (t (er hard? 'Smtlink=>save-user-hints "Smtlink hint seems in the wrong format ~p0.~%" user-hints)))))
+
+(verify-guards save-user-hints
+  :guard-debug t
+  :hints (("Goal"
+           :in-theory (enable smtlink-hint-syntax-fix
+                              smtlink-hint-syntax-p check-syntax)
+           :use ((:instance check-syntax-true-listp)))))
+
+(define merge-decl-list ((added-decls decl-listp) (master-adecls decl-alistp))
+  :returns (merged-decl-list decl-alistp)
+  :measure (len added-decls)
+  (b* ((added-decls (decl-list-fix added-decls))
+       (master-adecls (decl-alist-fix master-adecls))
+       ((unless (consp added-decls)) master-adecls)
+       ((cons first rest) added-decls)
+       ((decl d) first))
+    (merge-decl-list rest (hons-acons d.name first master-adecls))))
+
+(define merge-a-function ((fn func-p) (mfn func-p))
+  :returns (merged-fn func-p)
+  :verify-guards nil
+  (b* ((fn (func-fix fn))
+       (mfn (func-fix mfn))
+       ((func f) fn)
+       ((func mf) mfn)
+       ((unless (equal f.name mf.name))
+        (prog2$ (er hard? 'Smtlink=>merge-a-function "Trying to merge two functions
+  with different function names. Check definition for ~p0 and ~p1~%" fn mfn) (make-func)))
+        (formals-alist (make-alist-decl-list mf.formals))
+       (returns-alist (make-alist-decl-list mf.returns))
+       (long-formals
+        (with-fast-alist formals-alist
+          (merge-decl-list f.formals formals-alist)))
+       (short-formals (fast-alist-clean long-formals))
+       (long-returns
+        (with-fast-alist returns-alist
+          (merge-decl-list f.returns returns-alist)))
+       (short-returns (fast-alist-clean long-returns)))
+    (change-func mfn
+                 :formals (strip-cdrs short-formals)
+                 :guard (append f.guard mf.guard)
+                 :returns (strip-cdrs short-returns)
+                 :expansion-depth f.expansion-depth
+                 :uninterpreted f.uninterpreted)))
+
+(skip-proofs
+(verify-guards merge-a-function
+  :hints (("Goal"
+           :in-theory (enable decl-alistp))))
+)
+
+(define merge-functions ((added-funcs func-listp) (master-funcs func-alistp))
+  :returns (merged-functions func-alistp)
+  :measure (len added-funcs)
+  :hints (("Goal" :in-theory (enable func-alist-fix)))
+  :verify-guards nil
+  (b* ((added-funcs (func-alist-fix added-funcs))
+       (master-funcs (func-alist-fix master-funcs))
+       ((unless (consp added-funcs)) master-funcs)
+       ((cons first rest) added-funcs)
+       ((cons name fn) first)
+       (exist? (hons-get name master-funcs))
+       ((unless exist?)
+        (merge-functions rest (hons-acons name fn master-funcs)))
+       (mfn (cdr exist?))
+       (merged-fn (merge-a-function fn mfn)))
+    (merge-functions rest (hons-acons name merged-fn master-funcs))))
+
+(skip-proofs
+(verify-guards merge-functions
+  :hints (("Goal"
+           :in-theory (enable func-alist-fix func-alistp))))
+)
+
+(define merge-hints ((added-hint maybe-smtlink-hint-p) (master-hint smtlink-hint-p))
+  :returns (merged-hints smtlink-hint-p)
+  :verify-guards nil
+  (b* ((added-hint (maybe-smtlink-hint-fix added-hint))
+       (master-hint (smtlink-hint-fix master-hint))
+       ((if (equal added-hint nil)) master-hint)
+       ((smtlink-hint ah) added-hint)
+       ((smtlink-hint mh) master-hint)
+       (fn-alist (make-alist-fn-lst mh.functions)))
+    (change-smtlink-hint mh
+                         :functions (with-fast-alist fn-alist
+                                      (merge-functions ah.user-functions fn-alist))
+                         :user-functions ah.user-functions
+                         :hypotheses (append ah.hypotheses mh.hypotheses)
+                         :main-hint (append ah.main-hint mh.main-hint)
+                         :int-to-rat ah.int-to-rat
+                         :smt-fname ah.smt-fname
+                         :rm-file ah.rm-file
+                         :smt-params ah.smt-params
+                         :smt-cnf ah.smt-cnf)))
+
+(skip-proofs
+ (verify-guards merge-hints
+   :hints (("Goal"
+            :in-theory (enable))))
+ )
+
   (define combine-hints ((raw-user-hints smtlink-hint-syntax-p)
                          (hint smtlink-hint-p))
     :returns (combined-hint smtlink-hint-p)
-    :ignore-ok t
     (b* ((user-hints (smtlink-hint-syntax-fix raw-user-hints))
          (- (cw "Warning (Smtlink=>combine-hints): Smtlink hint syntax
     violated~% ~q0Therefore user provided Smtlink hint ignored.~%" raw-user-hints))
-         (hint (smtlink-hint-fix hint)))
-      hint))
+         (hint (smtlink-hint-fix hint))
+         (structured-user-hints (save-user-hints user-hints (make-smtlink-hint)))
+         (merged-hint (merge-hints structured-user-hints hint)))
+      merged-hint))
 
   (define process-hint ((cl pseudo-term-listp) (user-hint t))
     :returns (subgoal-lst pseudo-term-list-listp)
